theories/Decidability/Termination.v
@@ -1,0 +1,364 @@
+(** * LogRel.Decidability.Termination: the implementation always terminates on well-typed inputs. *)
+From Coq Require Import Nat Lia Arith.
+From Equations Require Import Equations.
+From LogRel.AutoSubst Require Import core unscoped Ast Extra.
+From LogRel Require Import Utils BasicAst Context Notations UntypedReduction DeclarativeTyping DeclarativeInstance GenericTyping NormalForms.
+From LogRel Require Import Validity LogicalRelation Fundamental DeclarativeSubst TypeConstructorsInj AlgorithmicTyping BundledAlgorithmicTyping Normalisation AlgorithmicConvProperties AlgorithmicTypingProperties.
+From LogRel.Decidability Require Import Functions Soundness Completeness.
+From PartialFun Require Import Monad PartialFun.
+
+Set Universe Polymorphism.
+
+Import DeclarativeTypingProperties.
+
+Section ConversionComplete.
+
+Let PTyEq (Γ : context) (A B : term) :=
+  forall v B',
+  [Γ |- B'] ->
+  domain conv (ty_state;Γ;v;A;B').
+Let PTyRedEq (Γ : context) (A B : term) :=
+  forall v B',
+  isType B' ->
+  [Γ |- B'] ->
+  domain conv (ty_red_state;Γ;v;A;B').
+Let PNeEq (Γ : context) (A t u : term) :=
+  forall v u',
+  whne u' ->
+  well_typed Γ u' ->
+  domain conv (ne_state;Γ;v;t;u').
+Let PNeRedEq (Γ : context) (A t u : term) :=
+  forall v u',
+  whne u' ->
+  well_typed Γ u' ->
+  domain conv (ne_red_state;Γ;v;t;u').
+Let PTmEq (Γ : context) (A t u : term) :=
+  forall u',
+  [Γ |- u' : A] ->
+  domain conv (tm_state;Γ;A;t;u').
+Let PTmRedEq (Γ : context) (A t u : term) :=
+  forall u',
+  whnf u' ->
+  [Γ |- u' : A] ->
+  domain conv (tm_red_state;Γ;A;t;u').
+
+Theorem _conv_terminates :
+  BundledConvInductionConcl PTyEq PTyRedEq PNeEq PNeRedEq PTmEq PTmRedEq.
+Proof.
+  subst PTyEq PTyRedEq PNeEq PNeRedEq PTmEq PTmRedEq.
+  apply BundledConvInduction.
+  - intros * ?? HA' [IH] **.
+    apply compute_domain.
+    simp conv.
+    cbn.
+    split.
+    1: eapply wh_red_complete ; now exists istype.
+    intros A''; split.
+    1: eapply wh_red_complete ; now exists istype.
+    intros B'' ; split.
+    2: easy.
+    assert [Γ |- B''].
+    {
+      eapply boundary_red_ty_r, subject_reduction_type.
+      2: now eapply red_sound.
+      eassumption.
+    }
+    replace A'' with A'.
+    1: apply (IH tt B'').
+    + eapply type_isType ; tea.
+      now eapply red_sound.
+    + eassumption. 
+    + eapply whred_det ; tea.
+      1: now eapply algo_conv_wh in HA' as [] ; gen_typing.
+      all: now eapply red_sound.
+  - intros * ? [IHA] ? [IHB] ? []%prod_ty_inv []%prod_ty_inv ? B' wB' HtyB'.
+    apply compute_domain.
+    simp conv.
+    destruct wB' as [|A'' B''| | |? wB'].
+    all: simp build_nf_ty_view2 ; cbn ; try easy.
+    2: now rewrite (whne_ty_view1 wB') ; cbn.
+    apply prod_ty_inv in HtyB' as [].
+    split.
+    2: intros [] ; cbn ; [|easy].
+    2: intros Hconv%implem_conv_sound%algo_conv_sound ; tea ; split ; [|easy].
+    + now apply (IHA tt A'').
+    + apply (IHB tt B'').
+      now eapply stability1.
+  - intros * ??? ? ? wB' ?.
+    apply compute_domain.
+    simp conv.
+    destruct wB' as [| | | |? wB'].
+    all: simp build_nf_ty_view2 ; cbn ; try easy.
+    now rewrite (whne_ty_view1 wB') ; cbn.
+  - intros * ??? ? ? wB' ?.
+    apply compute_domain.
+    simp conv.
+    destruct wB' as [| | | |? wB'].
+    all: simp build_nf_ty_view2 ; cbn ; try easy.
+    now rewrite (whne_ty_view1 wB') ; cbn.
+  - intros * ??? ? ? wB' ?.
+    apply compute_domain.
+    simp conv.
+    destruct wB' as [| | | |? wB'].
+    all: simp build_nf_ty_view2 ; cbn ; try easy.
+    now rewrite (whne_ty_view1 wB') ; cbn.
+  - intros * HM [IHM []] ??? ? ? wB' Hty.
+    apply compute_domain.
+    simp conv.
+    eapply algo_conv_wh in HM as [].
+    destruct wB' as [| | | |? wB'].
+    1-4: simp build_nf_ty_view2 ; cbn.
+    1-4: now unshelve erewrite whne_ty_view1 ; cbn.
+    erewrite whne_ty_view2 ; tea.
+    split.
+    2: intros [|] ; cbn ; easy.
+    eapply (IHM tt A) ; tea.
+    inversion Hty ; subst ; tea.
+    1-4: now inversion wB'.
+    now exists U.
+  - intros * ???? ? ? wu' ?.
+    apply compute_domain.
+    destruct wu' as [n'| | |].
+    all: simp conv ; cbn ; try easy.
+    destruct (Nat.eqb_spec n n') ; cbn.
+    2: easy.
+    split ; [|easy].
+    eexists.
+    now apply ctx_access_correct.
+  - intros ? ???? A B Hm [IHm []] ? [IHt] ??? ? u' wu' Hty.
+    apply compute_domain.
+    destruct wu' as [|m' t'| | ].
+    all: simp conv ; cbn ; try easy.
+    split.
+    + apply (IHm tt m') ; tea.
+      destruct Hty as [? (?&(?&?&[])&?)%termGen'].
+      now eexists.
+    + destruct Hty as [? (?&(?&?&[??Htym'])&?)%termGen'] ; subst.
+      intros [T|] ; cbn ; [|easy] ; intros [Hconvm?]%implem_conv_sound.
+      assert (T = tProd A B) by now eapply algo_conv_det.
+      subst.
+      apply algo_conv_sound in Hconvm as [?? Hgenm'].
+      2-3: now eexists ; boundary.
+      apply Hgenm' in Htym' as []%prod_ty_inj.
+      cbn.
+      split.
+      2: intros [|] ? ; cbn ; easy.
+      eapply (IHt t').
+      gen_typing.
+  - intros * Hn [IHn] ? [IHP] ? [IHz] ? [IHs] ??? ? u' wu' Hty.
+    apply compute_domain.
+    destruct wu' as [| |P'' hz'' hs'' n''| ].
+    all: simp conv ; cbn ; try easy.
+    destruct Hty as [? (?&[]&?)%termGen'].
+    split.
+    1: apply (IHn tt n'') ; tea ; now eexists.
+    intros [T|] ; cbn ; [|easy] ; intros [HconvT ?]%implem_conv_sound.
+    eapply algo_conv_det in HconvT as ->.
+    2: now apply Hn.
+    cbn.
+    split.
+    1: now apply (IHP tt P'').
+    intros [|] ; cbn ; [|easy] ; intros HconvP%implem_conv_sound%algo_conv_sound.
+    2-3: boundary.
+    split.
+    1:{
+      specialize (IHz hz'') ; apply IHz.
+      econstructor ; tea.
+      eapply typing_subst1.
+      2: now symmetry.
+      now do 2 econstructor.
+    }
+    assert (domain conv (tm_state; Γ; elimSuccHypTy P; hs; hs'')).
+    {
+      specialize (IHs hs'') ; apply IHs.
+      econstructor ; tea.
+      eapply elimSuccHypTy_conv ; tea.
+      now symmetry. 
+    }
+    intros [|] ; cbn.
+    2: now split.
+    intros ? ; split.
+    1: assumption.
+    now intros [|] ; cbn.
+  - intros * He [IHe] ? [IHP] ??? ? u' wu' Hty.
+    apply compute_domain.
+    destruct wu' as [| | | P'' e'' ].
+    all: simp conv ; cbn ; try easy.
+    destruct Hty as [? (?&[]&?)%termGen'].
+    split.
+    1: apply (IHe tt e'') ; tea ; now eexists.
+    intros [T|] ; cbn ; [|easy] ; intros [HconvT ?]%implem_conv_sound.
+    eapply algo_conv_det in HconvT as ->.
+    2: now apply He.
+    cbn.
+    split.
+    1: now apply (IHP tt P'').
+    intros [|] ; cbn ; easy.
+  - intros * ? [IHm] ?? ??? ? u' wu' Hty.
+    apply compute_domain.
+    simp conv ; cbn.
+    split.
+    2: intros [T|] ; cbn ; [|easy] ; intros []%implem_conv_sound%algo_conv_sound ; tea.
+    2: split ; [|easy].
+    + now apply (IHm tt u').
+    + eapply wh_red_complete.
+      exists istype.
+      boundary.
+  - intros * ??? Hconv [IHt'] ??? u' Hty.
+    apply compute_domain.
+    simp conv ; cbn.
+    split.
+    2: intros A'' [redA]%red_sound ; split.
+    3: intros t'' []%red_sound ; split.
+    4: intros u'' [redu]%red_sound ; split.
+    + eapply wh_red_complete.
+      exists istype.
+      boundary.
+    + eapply wh_red_complete.
+      now eexists (isterm _).
+    + eapply wh_red_complete.
+      now eexists (isterm _).
+    + assert (A'' = A').
+      {
+        eapply whred_det ; tea.
+        apply algo_conv_wh in Hconv as [].
+        gen_typing.
+      }
+      assert (t'' = t').
+      {
+        eapply whred_det ; tea.
+        now apply algo_conv_wh in Hconv as [].
+      }
+      subst.
+      eapply (IHt' u'') ; tea.
+      eapply subject_reduction in redu ; tea.
+      econstructor.
+      1: boundary.
+      eapply subject_reduction_type in redA as [] ; refold ; tea.
+      now boundary.
+    + easy.
+  - intros * ? [IHA] ? [IHB] ??? u' wu' Hty.
+    apply compute_domain.
+    simp conv build_nf_view3 build_nf_ty_view2.
+    eapply Uterm_isType in wu' ; tea.
+    destruct wu' as [ | A'' B'' | | | ? wu'] ; cycle -1.
+    1: rewrite (whne_ty_view1 wu').
+    all: cbn ; try easy.
+    eapply termGen' in Hty as (?&[]&?) ; subst.
+    split.
+    2: intros [|] ; cbn ; [|easy] ; intros ?%implem_conv_sound%algo_conv_sound.
+    3-4: boundary.
+    2: split.
+    + now apply (IHA A'').
+    + apply (IHB B'').
+      eapply stability1 ; tea.
+      1-2: boundary.
+      now constructor.
+    + now intros []. 
+  - intros * ??? u' wu' Hty.
+    apply compute_domain.
+    simp conv build_nf_view3 build_nf_ty_view2.
+    eapply Uterm_isType in wu' ; tea.
+    destruct wu' as [ | | | | ? wu'] ; cycle -1.
+    1: rewrite (whne_ty_view1 wu').
+    all: now cbn.
+  - intros * ??? u' wu' Hty.
+    apply compute_domain.
+    simp conv build_nf_view3 build_nf_ty_view2.
+    eapply nat_isNat in wu' ; tea.
+    destruct wu' as [ | | ? wu'] ; cycle -1.
+    1: rewrite (whne_nf_view1 wu').
+    all: now cbn.
+  - intros * ? [IHt] ??? u' wu' Hty.
+    apply compute_domain.
+    simp conv build_nf_view3 build_nf_ty_view2.
+    eapply nat_isNat in wu' ; tea.
+    destruct wu' as [ | u' | ? wu'] ; cycle -1.
+    1: rewrite (whne_nf_view1 wu').
+    all: cbn ; try easy.
+    split.
+    2: now intros [|] ; cbn.
+    eapply (IHt u').
+    now apply termGen' in Hty as (?&[]&?).
+  - intros * ??? u' wu' Hty.
+    apply compute_domain.
+    simp conv build_nf_view3 build_nf_ty_view2.
+    eapply Uterm_isType in wu' ; tea.
+    destruct wu' as [ | | | | ? wu'] ; cycle -1.
+    1: rewrite (whne_ty_view1 wu').
+    all: now cbn.
+  - intros * ?? ? [IHf] ??? u' wu' Hty.
+    apply compute_domain.
+    simp conv build_nf_view3 ; cbn.
+    split.
+    2: easy.
+    specialize (IHf (eta_expand u')).
+    apply IHf.
+    now eapply typing_eta'.
+  - intros * Hm [IHm []] Hpos ??? u' wu' Hu'.
+    apply compute_domain.
+    simp conv build_nf_view3.
+    eapply algo_conv_wh in Hm as [].
+    destruct Hpos as [[]| | | ].
+    + cbn.
+      simp build_nf_ty_view2.
+      unshelve erewrite whne_ty_view1 ; tea.
+      cbn.
+      eapply Uterm_isType in wu' ; tea.
+      destruct wu' as [ | | | | u' wu'] ; cbn ; try easy.
+      rewrite (whne_ty_view1 wu').
+      cbn.
+      split.
+      2: now intros [] ; cbn.
+      eapply (IHm tt u') ; tea.
+      now eexists.
+    + cbn.
+      unshelve erewrite whne_nf_view1 ; tea.
+      cbn.
+      eapply nat_isNat in wu' ; tea.
+      inversion wu'  as [| | u'' wu''] ; subst ; clear wu'.
+      all: cbn ; try easy.
+      rewrite (whne_nf_view1 wu'').
+      cbn.
+      split.
+      2: now intros [] ; cbn.
+      eapply (IHm tt u') ; tea.
+      now eexists.
+    + cbn.
+      unshelve erewrite whne_nf_view1 ; tea.
+      cbn.
+      eapply empty_isEmpty in wu' ; tea.
+      rewrite (whne_nf_view1 wu').
+      cbn.
+      split.
+      2: now intros [] ; cbn.
+      apply (IHm tt u') ; tea.
+      now eexists.
+    + unshelve erewrite whne_ty_view1 ; tea.
+      cbn.
+      eapply neutral_isNeutral in wu' ; tea.
+      split.
+      2: now intros [] ; cbn.
+      apply (IHm tt u') ; tea.
+      now eexists.
+  Qed.
+  
+  Corollary conv_terminates Γ A A' :
+    [Γ |-[de] A] ->
+    [Γ |-[de] A'] ->
+    forall v,
+    domain conv (ty_state;Γ;v;A;A').
+  Proof.
+    intros.
+    eapply _conv_terminates ; tea.
+    split.
+    4: eapply algo_conv_complete.
+    4: econstructor.
+    all: boundary.
+  Qed.
+
+End ConversionComplete.
+
+
+    
+
